---
title: "How to compute gradient (differentiation)"
date: 2019-10-29T20:07:07+01:00
draft: false
---

## Goal
Consider this simple equation:

$$ f(x,y,z) = ( x + y ) z $$

The goal of this article is to show you how Gorgonia can evaluate the gradient $\nabla f$ with

$$ \nabla f = [\frac{\partial f}{\partial x}, \frac{\partial f}{\partial y}, \frac{\partial f}{\partial z}] $$

### Explanation

To explain this, consider $q = x + y$.

Thanks to the chain rule, we can compute the gradient value at each step as illustrated here:

{{<mermaid align="left">}}
graph LR;
    x -->|$x=-2$<br>$\partial f/\partial x = -4$| add
    y -->|$y=5$<br>$\partial f/\partial y = -4$| add
    add -->|$q=3$<br>$\partial f/\partial q = -4$| mul
    z -->|$z=-4$<br>$\partial f/\partial z = 3$| mul
    mul(*) -->|$f=-12$<br>$1$| f
{{< /mermaid >}}


{{% notice info %}}
For more info on the gradient computation, please read this [article from cs231n](http://cs231n.github.io/optimization-2/) from Stanford.
{{% /notice %}}

We will represent this equation into an [exprgraph](/reference/exprgraph) and see how to ask Gorgonia to compute the gradient.

When the computation is done, each node will hold a [dual value](/reference/dualvalue) that will contain both the actual value and the derivative wrt to x.

for example, considering the node x:

```go
var x *gorgonia.Node
```

Once Gorgonia has evaluated the exprgraph, it is possible to extract the value of `x` and the value of the gradient $\frac{\partial f}{\partial x}$ by calling:

```go
xValue := x.Value() // -2
dfdx := x.Grad()    // -4
```

Let's see how to do that.

## Creating the equation

First, let's create the [exprgraph](/reference/exprgraph) that represents the equation.

{{% notice info %}}
If you want more info on this part, please read the [hello world](/tutorials/hello-world/) tutorial.
{{% /notice %}}

```go
g := gorgonia.NewGraph()

var x, y, z *gorgonia.Node
var err error

// define the expression
x = gorgonia.NewScalar(g, gorgonia.Float64, gorgonia.WithName("x"))
y = gorgonia.NewScalar(g, gorgonia.Float64, gorgonia.WithName("y"))
z = gorgonia.NewScalar(g, gorgonia.Float64, gorgonia.WithName("z"))
q, err := gorgonia.Add(x, y)
if err != nil {
    log.Fatal(err)
}
result, err := gorgonia.Mul(z, q)
if err != nil {
    log.Fatal(err)
}
```

And set some values:

```go
gorgonia.Let(x, -2.0)
gorgonia.Let(y, 5.0)
gorgonia.Let(z, -4.0)
```

### The gradient

There are two options to get the gradient:

* by using the [automatic differentiation](https://en.wikipedia.org/wiki/Automatic_differentiation) capability of the [LispMachine](/reference/lispmachine);
* by using the [symbolic differentiation](https://en.wikipedia.org/wiki/Computer_algebra) capability offered by Gorgonia;


#### The automatic differentiation

Automatic differentiation is only possible with the [LispMachine](/reference/lispmachine).
By default, lispmachine performs forward mode and backwards mode execution.

Therefore, calling the RunAll method is enough to get the result.
```go
m := gorgonia.newlispmachine(g)
defer m.close()
if err = m.RunAll(); err != nil {
    log.fatal(err)
}
```

The values and gradients can now be extracted:

```
fmt.Printf("x=%v;y=%v;z=%v\n", x.Value(), y.Value(), z.Value())
fmt.Printf("f(x,y,z) = %v\n", result.Value())

if xgrad, err := x.Grad(); err == nil {
    fmt.Printf("df/dx: %v\n", xgrad)
}
if ygrad, err := y.Grad(); err == nil {
    fmt.Printf("df/dy: %v\n", ygrad)
}
if xgrad, err := z.Grad(); err == nil {
    fmt.Printf("df/dx: %v\n", xgrad)
}
```

#### Symbolic differentiation

Another option is to use Symbolic differentiation.
Symbolic differentiation works by adding new nodes to the graphs. The new nodes represents holds the gradients wrt to the nodes passed as argument.

To create those new nodes, we use the [Grad()](https://godoc.org/gorgonia.org/gorgonia#Grad) function.

Grad takes a scalar cost node and a list of with-regards-to, and returns the gradient

Consider the following code:
```go
var grads Nodes
if grads, err = Grad(result,z, x, y); err != nil {
    log.Fatal(err)
}
```

`grads` in an array of `[]*gorgonia.Node` such as:

* `grads[0]` = $\frac{\partial f}{\partial z}$
* `grads[1]` = $\frac{\partial f}{\partial x}$
* `grads[2]` = $\frac{\partial f}{\partial y}$

The gradient is compatible with both [TapeMachine](/reference/tapemachine) and [LispMachine](/reference/lispmachine). But TapeMachine is much
faster.

```go
machine := gorgonia.NewTapeMachine(g)
defer machine.Close()
if err = machine.RunAll(); err != nil {
        log.Fatal(err)
}

fmt.Printf("result: %v\n", result.Value())
if zgrad, err := z.Grad(); err == nil {
        fmt.Printf("dz/dx: %v | %v\n", zgrad, grads[0].Value())
}

if xgrad, err := x.Grad(); err == nil {
        fmt.Printf("dz/dx: %v | %v\n", xgrad, grads[1].Value())
}

if ygrad, err := y.Grad(); err == nil {
        fmt.Printf("dz/dy: %v | %v\n", ygrad, grads[2].Value())
}
```

## Full code

```go
func main() {
	g := gorgonia.NewGraph()

	var x, y, z *gorgonia.Node
	var err error

	// define the expression
	x = gorgonia.NewScalar(g, gorgonia.Float64, gorgonia.WithName("x"))
	y = gorgonia.NewScalar(g, gorgonia.Float64, gorgonia.WithName("y"))
	z = gorgonia.NewScalar(g, gorgonia.Float64, gorgonia.WithName("z"))
	q, err := gorgonia.Add(x, y)
	if err != nil {
		log.Fatal(err)
	}
	result, err := gorgonia.Mul(z, q)
	if err != nil {
		log.Fatal(err)
	}

	// set initial values then run
	gorgonia.Let(x, -2.0)
	gorgonia.Let(y, 5.0)
	gorgonia.Let(z, -4.0)

	// by default, lispmachine performs forward mode and backwards mode execution
	m := gorgonia.newlispmachine(g)
	defer m.close()
	if err = m.runall(); err != nil {
		log.fatal(err)
	}

	fmt.Printf("x=%v;y=%v;z=%v\n", x.Value(), y.Value(), z.Value())
	fmt.Printf("f(x,y,z)=(x+y)*z\n")
	fmt.Printf("f(x,y,z) = %v\n", result.Value())

	if xgrad, err := x.Grad(); err == nil {
		fmt.Printf("df/dx: %v\n", xgrad)
	}

	if ygrad, err := y.Grad(); err == nil {
		fmt.Printf("df/dy: %v\n", ygrad)
	}
	if xgrad, err := z.Grad(); err == nil {
		fmt.Printf("df/dz: %v\n", xgrad)
	}
}
```

which gives:

```text
$ go run main.go
x=-2;y=5;z=-4
f(x,y,z)=(x+y)*z
f(x,y,z) = -12
df/dx: -4
df/dy: -4
df/dz: 3
```
